start proving memory safety for the encoding function

code/experimental/rsa/RSA.fst
@@ -15,6 +15,8 @@ open MGF
 module U32 = FStar.UInt32
 module U8 = FStar.UInt8
 
+#set-options "--lax"
+
 inline_for_extraction let zero_8 = 0uy
 inline_for_extraction let hLen = 32ul
 
@@ -40,99 +42,137 @@ let xordb len b1 b2 =
 	C.Loops.in_place_map2 b1 b2 len (fun x y -> U8.(x ^^ y))
 
 val pss_encode:
-	saltLen:U32.t ->
-	modBits:U32.t{U32.v (get_length_em modBits) >= U32.(v (saltLen +^ hLen +^ 2ul))} ->
-	msg:uint8_p -> len:U32.t{U32.v len = length msg} ->
-	salt:uint8_p{length salt = U32.v saltLen} ->
-	em:uint8_p{length em = U32.v (get_length_em modBits)} -> Stack unit
+	saltLen:blen ->
+	modBits:U32.t{U32.v modBits > 0 /\ U32.v saltLen + 32 + 2 <= U32.v (get_length_em modBits)} ->
+	len:U32.t ->
+	salt:lbytes saltLen ->
+	msg:uint8_p{length msg = U32.v len /\ length msg < pow2 61 /\ disjoint msg salt} ->
+	em:lbytes (get_length_em modBits){disjoint salt em /\ disjoint salt msg} -> Stack unit
 	(requires (fun h -> live h msg /\ live h em /\ live h salt))
-	(ensures (fun h0 _ h1 -> live h0 msg /\ live h0 em /\  live h0 salt /\ live h1 em /\ modifies_1 em h0 h1))
-let pss_encode saltLen modBits msg len salt em =
+	(ensures (fun h0 _ h1 -> live h0 msg /\ live h0 em /\  live h0 salt /\ 
+		live h1 msg /\ live h1 salt /\ live h1 em /\ modifies_1 em h0 h1))
+
+//#reset-options "--z3rlimit 15"
+
+let pss_encode saltLen modBits len salt msg em =
 	push_frame();
-	let mHash = create zero_8 hLen in
-	hash_sha256 mHash len msg;
-	let emBits = U32.(modBits -^ 1ul) in
 	let emLen = get_length_em modBits in
-	let m1_size = U32.(8ul +^ hLen +^ saltLen) in
-	let m1 = create zero_8 m1_size in
+	(**) assert(length em = U32.v emLen);
+	(**) assert(U32.v saltLen + 32 + 2 <= U32.v emLen);
+	let m1_size = U32.(8ul +^ 32ul +^ saltLen) in
+	(**) assert(0 < U32.v emLen - 32 - 1);
+	let db_size = U32.(emLen -^ 32ul -^ 1ul) in
+
+	let mHash = create 0uy 32ul in
+	let m1 = create 0uy m1_size in
+	let m1Hash = create 0uy 32ul in
+	let db = create 0uy db_size in
+	let dbMask = create 0uy db_size in
+	
+	hash_sha256 mHash len msg;
 	(* first 8 elements should be 0x00 *)
-	blit mHash 0ul m1 8ul hLen;
-	blit salt 0ul m1 U32.(8ul +^ hLen) saltLen;
-	let m1Hash = create zero_8 hLen in
+	blit mHash 0ul m1 8ul 32ul;
+	blit salt 0ul m1 U32.(8ul +^ 32ul) saltLen;
 	hash_sha256 m1Hash m1_size m1;
 
-	let db_size = U32.(emLen -^ hLen -^ 1ul) in
-	let db = create zero_8 db_size in
-	let ind_1 = U32.(emLen -^ saltLen -^ hLen -^ 2ul) in
+	(**) assert(0 <= U32.v emLen - (U32.v saltLen) - 32 - 2); 
+	let ind_1 = U32.(emLen -^ saltLen -^ 32ul -^ 2ul) in
+	(**) assume(U32.v ind_1 < length db);
 	db.(ind_1) <- 1uy;
+	(**) assume(U32.v ind_1 + 1 < length db);
+	(**) assume(U32.v ind_1 + 1 + U32.v saltLen < length db);
 	blit salt 0ul db U32.(ind_1 +^ 1ul) saltLen;
-
-	let dbMask = create zero_8 db_size in
 	mgf_sha256 m1Hash db_size dbMask;
-
+	
 	xordb db_size db dbMask;
-	let zeroL = U32.(8ul *^ emLen -^ emBits) in
-	db.(0ul) <- U8.(db.(0ul) &^ (0xffuy >>^ zeroL));
-
+	(**) assume(0 < 8 * (U32.v emLen) - (U32.v modBits - 1) /\
+		       8 * (U32.v emLen) - (U32.v modBits - 1) < pow2 32);
+	let zeroL = U32.(8ul *^ emLen -^ (modBits -^ 1ul)) in
+	let db_0 = db.(0ul) in
+	(**) assume(U32.v zeroL < pow2 8);
+	(**) assert(255 < pow2 8);
+	let tmp = U8.(255uy >>^ zeroL) in
+	db.(0ul) <- U8.(db_0 &^ tmp);
 	blit db 0ul em 0ul db_size;
 	blit m1Hash 0ul em db_size hLen;
 	upd em U32.(emLen -^ 1ul) 0xbcuy;
 	pop_frame()
 
+
 val pss_verify:
 	saltLen:U32.t ->
-	modBits:U32.t{U32.v (get_length_em modBits) >= U32.(v (saltLen +^ hLen +^ 2ul))} ->
-	em:uint8_p{length em = U32.v (get_length_em modBits)} ->
-	msg:uint8_p -> len:U32.t{U32.v len = length msg} -> Stack bool
+	modBits:U32.t{U32.v modBits > 0 /\ U32.v saltLen + 32 + 2 <= U32.v (get_length_em modBits)} ->
+	len:U32.t ->
+	em:lbytes (get_length_em modBits) ->
+	msg:uint8_p{length msg = U32.v len /\ length msg < pow2 61 /\ disjoint msg em} -> Stack bool
 	(requires (fun h -> live h msg /\ live h em))
-	(ensures (fun h0 _ h1 -> live h0 msg /\ live h0 em /\ live h1 msg /\ live h1 em))
-let pss_verify saltLen modBits em msg len =
+	(ensures (fun h0 _ h1 -> live h0 msg /\ live h0 em /\ 
+		live h1 msg /\ live h1 em /\ modifies_0 h0 h1))
+
+#reset-options "--z3rlimit 15"
+
+let pss_verify saltLen modBits len em msg =
 	push_frame();
 	let emLen = get_length_em modBits in
-	let m1_size = U32.(8ul +^ hLen +^ saltLen) in
-	let pad_size = U32.(emLen -^ saltLen -^ hLen -^ 1ul) in
-	let db_size = U32.(emLen -^ hLen -^ 1ul) in
+	let m1_size = U32.(8ul +^ 32ul +^ saltLen) in
+	let pad_size = U32.(emLen -^ saltLen -^ 32ul -^ 1ul) in
+	let db_size = U32.(emLen -^ 32ul -^ 1ul) in
 
-	let mHash = create zero_8 hLen in
-	let m1Hash' = create zero_8 hLen in
-	let m1 = create zero_8 m1_size in
-	let pad2 = create zero_8 pad_size in
-	let dbMask = create zero_8 db_size in
+	let mHash = create 0uy 32ul in
+	let m1 = create 0uy m1_size in
+	let m1Hash' = create 0uy 32ul in
+	let pad2 = create 0uy pad_size in
+	let dbMask = create 0uy db_size in
 
 	hash_sha256 mHash len msg;
 	let res =
-	if not (U8.(em.(U32.(emLen -^ 1ul)) =^ 0xbcuy)) then false else (
-	let maskedDB = sub em 0ul db_size in
-	let m1Hash = sub em db_size hLen in
-	let zeroL = U32.(8ul *^ emLen -^ (modBits -^ 1ul)) in
-	let tmp = U8.(maskedDB.(0ul) &^ (0xffuy <<^ U32.(8ul -^ zeroL))) in
-	if not (U8.(tmp =^ 0x00uy)) then false else (
-	mgf_sha256 m1Hash db_size dbMask;
-	xordb db_size maskedDB dbMask;
-	maskedDB.(0ul) <- U8.(maskedDB.(0ul) &^ (0xffuy >>^ zeroL));
-	upd pad2 U32.(pad_size -^ 1ul) 0x01uy;
+		if not (U8.(em.(U32.(emLen -^ 1ul)) =^ 0xbcuy)) then false 
+		else begin 
+			let maskedDB = sub em 0ul db_size in
+			let m1Hash = sub em db_size hLen in
+			let zeroL = U32.(8ul *^ emLen -^ (modBits -^ 1ul)) in
+			let tmp = U8.(maskedDB.(0ul) &^ (0xffuy <<^ U32.(8ul -^ zeroL))) in
+			if not (U8.(tmp =^ 0x00uy)) then false 
+			else begin
+				mgf_sha256 m1Hash db_size dbMask;
+				xordb db_size maskedDB dbMask;
+				maskedDB.(0ul) <- U8.(maskedDB.(0ul) &^ (0xffuy >>^ zeroL));
+				upd pad2 U32.(pad_size -^ 1ul) 0x01uy;
 
-	let pad = sub maskedDB 0ul pad_size in
-	if not (eqb pad pad2 pad_size) then false else (
-	let salt = sub maskedDB pad_size saltLen in
-	(* first 8 elements should be 0x00 *)
-	blit mHash 0ul m1 8ul hLen;
-	blit salt 0ul m1 U32.(8ul +^ hLen) saltLen;
-	hash_sha256 m1Hash' m1_size m1;
-	eqb m1Hash m1Hash' hLen))) in
+				let pad = sub maskedDB 0ul pad_size in
+				if not (eqb pad pad2 pad_size) then false 
+				else begin
+					let salt = sub maskedDB pad_size saltLen in
+					(* first 8 elements should be 0x00 *)
+					blit mHash 0ul m1 8ul hLen;
+					blit salt 0ul m1 U32.(8ul +^ hLen) saltLen;
+					hash_sha256 m1Hash' m1_size m1;
+					eqb m1Hash m1Hash' hLen
+					end
+				end 
+			end in
 	pop_frame();
 	res
 
+(* ADD disjointness for skey ? *)
 val rsa_sign:
 	saltLen:U32.t ->
-	modBits:U32.t{U32.v (get_length_em modBits) >= U32.(v (saltLen +^ hLen +^ 2ul))} ->
-	skeyBits:U32.t -> msgLen:U32.t ->
-	msg:uint8_p{length msg = U32.v msgLen} ->
+	modBits:U32.t{U32.v saltLen + 32 + 2 <= U32.v (get_length_em modBits)} ->
+	skeyBits:U32.t{U32.v skeyBits <= U32.v modBits} -> msgLen:U32.t ->
+	msg:uint8_p{length msg = U32.v msgLen /\ length msg < pow2 61} ->
 	skey:rsa_privkey ->
-	salt:uint8_p{length salt = U32.v saltLen} ->
-	sgnt:uint8_p{length sgnt = U32.v (bits_to_text modBits)} -> Stack unit
-	(requires (fun h -> live h msg /\ live h salt /\ live h sgnt))
-	(ensures (fun h0 _ h1 -> live h0 msg /\ live h0 salt /\ live h0 sgnt /\ live h1 sgnt /\ modifies_1 sgnt h0 h1))
+	salt:lbytes saltLen{disjoint salt msg} ->
+	sgnt:lbytes (bits_to_text modBits){disjoint sgnt msg /\ disjoint sgnt salt} -> Stack unit
+	(requires (fun h -> let pkey = Mk_rsa_privkey?.pkey skey in
+			live h msg /\ live h salt /\ live h sgnt /\ 
+			live h (Mk_rsa_privkey?.d skey) /\ live h (Mk_rsa_pubkey?.n pkey) /\ live h (Mk_rsa_pubkey?.e pkey)))
+	(ensures (fun h0 _ h1 ->
+			let pkey = Mk_rsa_privkey?.pkey skey in
+			live h0 msg /\ live h0 salt /\ live h0 sgnt /\ live h1 msg /\ live h1 salt /\ live h1 sgnt /\
+			live h0 (Mk_rsa_privkey?.d skey) /\ live h0 (Mk_rsa_pubkey?.n pkey) /\ live h0 (Mk_rsa_pubkey?.e pkey) /\
+			live h1 (Mk_rsa_privkey?.d skey) /\ live h1 (Mk_rsa_pubkey?.n pkey) /\ live h1 (Mk_rsa_pubkey?.e pkey) /\
+			modifies_1 sgnt h0 h1))
+
 let rsa_sign saltLen modBits skeyBits msgLen msg skey salt sgnt =
 	push_frame();
 	let k = bits_to_text modBits in
@@ -141,8 +181,8 @@ let rsa_sign saltLen modBits skeyBits msgLen msg skey salt sgnt =
 	let n = Mk_rsa_pubkey?.n pkey in
 
 	let emLen = get_length_em modBits in
-	let em = create zero_8 emLen in
-	pss_encode saltLen modBits msg msgLen salt em;
+	let em = create 0uy emLen in
+	pss_encode saltLen modBits msgLen salt msg em;
 	let mLen = get_size_nat emLen in
 	let m = create 0uL mLen in
 	text_to_nat emLen em m;
@@ -155,15 +195,20 @@ let rsa_sign saltLen modBits skeyBits msgLen msg skey salt sgnt =
 	nat_to_text k s sgnt;
 	pop_frame()
 
+
 val rsa_verify:
 	saltLen:U32.t ->
-	modBits:U32.t{U32.v (get_length_em modBits) >= U32.(v (saltLen +^ hLen +^ 2ul))} ->
-	msgLen:U32.t -> pkeyBits:U32.t ->
-	sgnt:uint8_p{length sgnt = U32.v (bits_to_text modBits)} ->
+	modBits:U32.t{U32.v modBits > 0 /\ U32.v saltLen + 32 + 2 <= U32.v (get_length_em modBits)} ->
+	msgLen:U32.t -> pkeyBits:U32.t{U32.v pkeyBits <= U32.v modBits} ->
+	sgnt:lbytes (bits_to_text modBits) ->
 	pkey:rsa_pubkey ->
-	msg:uint8_p{length msg = U32.v msgLen} -> Stack bool
-	(requires (fun h -> live h msg /\ live h sgnt))
-	(ensures (fun h0 _ h1 -> live h0 msg /\ live h0 sgnt /\ live h1 msg /\ live h1 sgnt))
+	msg:uint8_p{length msg = U32.v msgLen /\ length msg < pow2 61 /\ disjoint msg sgnt} -> Stack bool
+	(requires (fun h -> live h msg /\ live h sgnt /\ live h (Mk_rsa_pubkey?.e pkey) /\ live h (Mk_rsa_pubkey?.n pkey)))
+	(ensures (fun h0 _ h1 -> live h0 msg /\ live h0 sgnt /\ live h1 msg /\ live h1 sgnt /\
+			live h0 (Mk_rsa_pubkey?.e pkey) /\ live h0 (Mk_rsa_pubkey?.n pkey) /\
+			live h1 (Mk_rsa_pubkey?.e pkey) /\ live h1 (Mk_rsa_pubkey?.n pkey) /\ 
+			modifies_0 h0 h1))
+
 let rsa_verify saltLen modBits msgLen pkeyBits sgnt pkey msg =
 	push_frame();
 	let e = Mk_rsa_pubkey?.e pkey in
@@ -181,8 +226,8 @@ let rsa_verify saltLen modBits msgLen pkeyBits sgnt pkey msg =
 	let m = create 0uL mLen in
 	mod_exp modBits signLen pkeyBits mLen n s e m;
 
-	let em = create zero_8 emLen in
+	let em = create 0uy emLen in
 	nat_to_text emLen m em;
-	let res = pss_verify saltLen modBits em msg msgLen in
+	let res = pss_verify saltLen modBits msgLen em msg in
 	pop_frame();
 	res
